CloseLemmas.v
@@ -1,0 +1,62 @@
+Require Import Termination.Tactics.
+Require Import Termination.Sets.
+Require Import Termination.Syntax.
+Require Import Termination.SubstitutionLemmas.
+Require Import Termination.FVLemmas.
+Require Import Termination.FVLemmasLists.
+Require Import Termination.ListUtils.
+Require Import Termination.AssocList.
+
+Lemma close_nothing:
+  forall x t k,
+    ~(x ∈ pfv t term_var) ->
+    close k t x = t.
+Proof.
+  induction t;
+    repeat step || tequality || t_listutils.
+Qed.
+
+Lemma close_nothing2:
+  forall x t k,
+    pfv t term_var = nil ->
+    close k t x = t.
+Proof.
+  intros; apply close_nothing; repeat step || rewrite_any.
+Qed.
+
+Lemma substitute_close:
+  forall t l tag x k,
+    ~(x ∈ support l) ->
+    pclosed_mapping l term_var ->
+    psubstitute (close k t x) l tag = close k (psubstitute t l tag) x.
+Proof.
+  induction t;
+    repeat step || tequality || t_lookup || rewrite close_nothing2 by (steps; eauto with bfv).
+Qed.
+
+Lemma tclose_nothing:
+  forall x t k,
+    ~(x ∈ pfv t type_var) ->
+    tclose k t x = t.
+Proof.
+  induction t;
+    repeat step || tequality || t_listutils.
+Qed.
+
+Lemma tclose_nothing2:
+  forall x t k,
+    pfv t type_var = nil ->
+    tclose k t x = t.
+Proof.
+  intros; apply tclose_nothing; repeat step || rewrite_any.
+Qed.
+
+Lemma substitute_tclose:
+  forall t l tag x k,
+    ~(x ∈ support l) ->
+    pclosed_mapping l type_var ->
+    psubstitute (tclose k t x) l tag = tclose k (psubstitute t l tag) x.
+Proof.
+  induction t;
+    repeat step || tequality || t_lookup || rewrite tclose_nothing2 by (steps; eauto with bfv).
+Qed.
