FVLemmasClose.v
@@ -1,0 +1,96 @@
+Require Import Coq.Strings.String.
+Require Import Coq.Lists.List.
+Require Import Coq.Init.Datatypes.
+Require Import Coq.Arith.PeanoNat.
+
+Require Import Termination.Syntax.
+Require Import Termination.Tactics.
+Require Import Termination.ListUtils.
+Require Import Termination.AssocList.
+Require Import Termination.Sets.
+Require Import Termination.SetLemmas.
+Require Import Termination.FVLemmas.
+
+Lemma fv_close1:
+  forall t k x,
+    x ∈ pfv (close k t x) term_var ->
+    False.
+Proof.
+  induction t;
+    repeat step || t_listutils; eauto.
+Qed.
+
+Lemma fv_close2:
+  forall t k x y,
+    y ∈ pfv (close k t x) term_var ->
+    y <> x /\ y ∈ pfv t term_var.
+Proof.
+  induction t;
+    repeat match goal with
+           | _ => step || t_listutils || instantiate_any
+           end;
+    eauto 3 using fv_close1;
+    eauto 5 with beapply_any.
+Qed.
+
+Lemma fv_close3:
+  forall t k x y,
+    y ∈ pfv (tclose k t x) term_var ->
+    y ∈ pfv t term_var.
+Proof.
+  induction t;
+    repeat match goal with
+           | _ => step || t_listutils || instantiate_any
+           end;
+    eauto with beapply_any.
+Qed.
+
+Lemma tfv_close1:
+  forall t k x,
+    x ∈ pfv (tclose k t x) type_var ->
+    False.
+Proof.
+  induction t;
+    repeat step || t_listutils; eauto.
+Qed.
+
+Lemma tfv_close2:
+  forall t k x y,
+    y ∈ pfv (tclose k t x) type_var ->
+    y <> x /\ y ∈ pfv t type_var.
+Proof.
+  induction t;
+    repeat match goal with
+           | _ => step || t_listutils || instantiate_any
+           end;
+    eauto 3 using tfv_close1;
+    eauto 5 with beapply_any.
+Qed.
+
+Lemma tfv_close3:
+  forall t k x y,
+    y ∈ pfv (close k t x) type_var ->
+    y ∈ pfv t type_var.
+Proof.
+  induction t;
+    repeat match goal with
+           | _ => step || t_listutils || instantiate_any
+           end;
+    eauto with beapply_any.
+Qed.
+
+Ltac t_fv_close :=
+  match goal with
+  | H: _ ∈ pfv (close _ _ _) term_var |- _ =>
+    poseNew (Mark H "t_fv_close");
+    unshelve epose proof (fv_close2 _ _ _ _ H)
+  | H: _ ∈ pfv (tclose _ _ _) term_var |- _ =>
+    poseNew (Mark H "t_fv_close");
+    unshelve epose proof (fv_close3 _ _ _ _ H)
+  | H: _ ∈ pfv (tclose _ _ _) type_var |- _ =>
+    poseNew (Mark H "t_fv_close");
+    unshelve epose proof (tfv_close2 _ _ _ _ H)
+  | H: _ ∈ pfv (tclose _ _ _) type_var |- _ =>
+    poseNew (Mark H "t_fv_close");
+    unshelve epose proof (tfv_close3 _ _ _ _ H)
+  end.
