WFLemmasClose.v
@@ -1,0 +1,50 @@
+Require Import Coq.Strings.String.
+Require Import Omega.
+
+Require Import Termination.Syntax.
+Require Import Termination.Tactics.
+Require Import Termination.AssocList.
+Require Import Termination.Sets.
+Require Import Termination.ListUtils.
+Require Import Termination.WellFormed.
+Require Import Termination.WFLemmas.
+
+Open Scope string_scope.
+Open Scope list_scope.
+
+Lemma wf_close:
+  forall t k x,
+    wf t k ->
+    wf (close k t x) (S k).
+Proof.
+  induction t; steps.
+Qed.
+
+Lemma wf_tclose:
+  forall t i j x,
+    wf t i ->
+    wf (tclose j t x) i.
+Proof.
+  induction t; steps.
+Qed.
+
+Lemma twf_tclose:
+  forall T k X,
+    twf T k ->
+    twf (tclose k T X) (S k).
+Proof.
+  induction T; steps.
+Qed.
+
+Lemma twf_close:
+  forall t i j x,
+    twf t i ->
+    twf (close j t x) i.
+Proof.
+  induction t; steps.
+Qed.
+
+Hint Resolve wf_close: bwf.
+Hint Resolve twf_tclose: btwf.
+Hint Resolve wf_tclose: bwf.
+Hint Resolve twf_close: btwf.
